ClassicalLanguage/de_hoare.lean
@@ -6,6 +6,35 @@ import ClassicalLanguage.de_BSOS
 def hoare(P: Cond)(prog: Program)(Q: Cond): Prop :=
     ∀sStart sFin: State, evalC P sStart → BSOS sStart prog sFin → evalC Q sFin
 
+lemma strengthPostCond (Qn: Cond)(P Q: Cond)(prog: Program):
+    fol Q Qn → hoare P prog Q → hoare P prog Qn := by
+  intro stronger
+  intro hoare1
+  rw [hoare]
+  intro sStart sFin
+  intro preCond
+  intro trans
+  have postCond: evalC Q sFin := by
+    apply hoare1 sStart sFin
+    apply preCond
+    apply trans
+  clear preCond trans sStart hoare1 prog P
+  apply stronger sFin
+  apply postCond
+
+lemma weakenPreCond (Pn: Cond)(P Q: Cond)(prog: Program):
+    fol Pn P → hoare P prog Q → hoare Pn prog Q := by
+    intro weaker
+    intro hoare1
+    rw [hoare]
+    intro sStart sFin
+    intro preCond
+    intro trans
+    apply hoare1 sStart sFin
+    apply weaker sStart
+    apply preCond
+    apply trans
+
 theorem hoareSkip(P: Cond): hoare P Program.skip P := by
   rw [hoare]
   intro sStart sFin
@@ -46,17 +75,6 @@ theorem hoareSeq(P R Q: Cond)(p1 p2: Program):
     apply preCond
     apply trans1
     apply trans2
-
-theorem hoareAssign(name: String)(expr: Expr)(Q: Cond):
-  hoare (replC Q name expr) (Program.assign name expr) Q := by
-  rw [hoare]
-  intro sStart sFin
-  rw [condReplacement]
-  intro precond
-  intro trans
-  cases trans
-  case assign =>
-    apply precond
 
 theorem hoareIf(P Q: Cond)(cond: Cond)(pt pf: Program):
   hoare P pt Q → hoare P pf Q → hoare P (Program.iff cond pt pf) Q := by
